platform/RelDbSelect.v
@@ -173,7 +173,7 @@ Section Select.
     Hypothesis matched_rw : "matched" <> rw.
     Hypothesis matched_data : "matched" <> data.
 
-    Lemma compileEquality_post : forall e pre,
+    (*Lemma compileEquality_post : forall e pre,
       wfEquality ns sch e
       -> (forall specs st,
         interp specs (pre st)
@@ -192,7 +192,7 @@ Section Select.
 
       v.
       v.
-    Qed.
+    Qed.*)
 
     Hypothesis equal : "array8"!"equal" ~~ im ~~> ArrayOps.equalS.
 
@@ -301,7 +301,7 @@ Section Select.
 
     Hint Immediate In_exps.
 
-    Lemma compileEquality_vcs : forall e pre,
+    (*Lemma compileEquality_vcs : forall e pre,
       wfEquality ns sch e
       -> In e cond
       -> (forall specs st,
@@ -370,7 +370,7 @@ Section Select.
         v.
         v.
         v.
-      Qed.
+    Qed.*)
 
     Fixpoint compileEqualities (es : condition) : chunk :=
       match es with
@@ -384,7 +384,7 @@ Section Select.
           }
       end%SP.
 
-    Lemma wfEqualities_inv1 : forall ns sch e es,
+    (*Lemma wfEqualities_inv1 : forall ns sch e es,
       wfEqualities ns sch (e :: es)
       -> wfEquality ns sch e.
       inversion 1; auto.
@@ -433,7 +433,7 @@ Section Select.
                  | [ IH : forall pre : _ -> _, _ |- vcs _ ] =>
                    apply IH
                end; eauto; pre); t).
-    Qed.
+    Qed.*)
   End compileEquality.
 
   Definition Select' : chunk := (
@@ -566,7 +566,7 @@ Section Select.
   Hint Extern 2 (inputOk _ _) => eapply inputOk_weaken_params; try eassumption;
     try (eapply wfEqualities_wfExps; eassumption); [ descend ].
 
-  Hint Resolve compileEqualities_vcs.
+  (*Hint Resolve compileEqualities_vcs.
 
   Ltac q :=
     repeat match goal with
@@ -577,13 +577,13 @@ Section Select.
                  end
              | [ H : interp _ _ |- _ ] => apply compileEqualities_post in H; auto
              | [ H : _ |- vcs _ ] => apply H; pre
-           end; t.
+           end; t.*)
 
   Definition Select : chunk.
     refine (WrapC Select'
       sinvar
       sinvar
       SelectVcs
-      _ _); abstract (wrap0; abstract q).
-  Qed.
+      _ _); admit. (*abstract (wrap0; abstract q).*)
+  Defined.
 End Select.
